ok

Lamcalc/Basics.lean
@@ -1,5 +1,3 @@
-import Mathlib.Tactic
-
 class Ids (t : Type) where
   ids : Nat -> t
 
@@ -13,10 +11,12 @@ export Ids (ids)
 export Rename (rename)
 export Subst (subst)
 
+@[simp]
 def scons {T} (s : T) (σ : Nat -> T) : Nat -> T
   | 0 => s
   | x+1 => σ x
 
+@[simp]
 def funcomp {A B C} (f : A -> B) (g : B -> C) : A -> C :=
   fun x => g (f x)
 
@@ -29,25 +29,31 @@ infixr:55 " .: " => scons
 notation:max s:2 ".[" σ:2 "]" => subst σ s
 notation:max s:2 ".[" t:2 "/]" => subst (t .: ids) s
 
-def upren (ξ : Nat -> Nat) : Nat -> Nat :=
-  0 .: ξ @@@ Nat.succ
-
 def ren {T} [Ids T] (ξ : Nat -> Nat) : Nat -> T :=
   ξ @@@ ids
 
+def shift {T} [Ids T] : Nat -> T :=
+  ren Nat.succ
+
+def upren (ξ : Nat -> Nat) : Nat -> Nat :=
+  0 .: ξ @@@ Nat.succ
+
 def up {T} [Ids T] [Rename T] (σ : Nat -> T) : Nat -> T :=
-  ids 0 .: σ @@@ rename Nat.succ
+  ids 0 .: (σ @@@ rename Nat.succ)
 
 def upn {T} [Ids T] [Rename T] (n : Nat) : (Nat -> T) -> Nat -> T :=
-  up^[n]
+  n.repeat up
 
-lemma upren0 (ξ : Nat -> Nat) : upren ξ 0 = 0 := rfl
-lemma up0 {T} [Ids T] [Rename T] (σ : Nat -> T) : up σ 0 = ids 0 := rfl
-lemma upn0 {T} [Ids T] [Rename T] σ : @upn T _ _ 0 σ = σ := rfl
-lemma upn1 {T} [Ids T] [Rename T] (n : Nat) σ : @upn T _ _ (n + 1) σ = upn n (up σ) := rfl
-attribute [simp] upren0 up0 upn0 upn1
+@[simp] theorem upren0 (ξ : Nat -> Nat) : upren ξ 0 = 0 := by rfl
+@[simp] theorem up0 {T} [Ids T] [Rename T] (σ : Nat -> T) : up σ 0 = ids 0 := by rfl
 
-lemma id_comp {A B} (f : A -> B) : f @@@ id = f := by rfl
-lemma comp_id {A B} (f : A -> B) : id @@@ f = f := by rfl
-lemma comp_assoc {A B C D} (f : A -> B) (g : B -> C) (h : C -> D) :
-  f @@@ (g @@@ h) = (f @@@ g) @@@ h := by rfl
+@[simp] theorem up1 {T} [Ids T] [Rename T] (σ : Nat -> T) : up σ (n + 1) = rename Nat.succ (σ n) := by rfl
+@[simp] theorem upn0 {T} [Ids T] [Rename T] σ : @upn T _ _ 0 σ = σ := by rfl
+@[simp] theorem upn1 {T} [Ids T] [Rename T] (n : Nat) σ : @upn T _ _ (n + 1) σ = upn n (up σ) := by
+  induction n with
+  | zero => simp[upn, Nat.repeat]
+  | succ n ih =>
+    simp[upn, Nat.repeat]
+    rw [<-upn]
+    rw [<-ih]
+    simp[upn, Nat.repeat]
