Lamcalc/ARS.lean
@@ -1,5 +1,3 @@
-import Mathlib.Tactic
-
 namespace ARS
 
 section ars_def
@@ -21,8 +19,6 @@ inductive conv (x : T) : T -> Prop where
 | SE  {y z} : conv x y -> e y z -> conv x z
 | SEi {y z} : conv x y -> e z y -> conv x z
 
-attribute [aesop unsafe] star.R conv.R
-
 def com (R S : Rel T) := ∀ {x y z}, R x y -> S x z -> ∃ u, S y u ∧ R z u
 def joinable (R : Rel T) x y := ∃ z, R x z ∧ R y z
 def diamond := ∀ {x y z}, e x y -> e x z -> ∃ u, e y u ∧ e z u
@@ -33,100 +29,100 @@ end ars_def
 section ars_lemmas
 variable {T : Type} {e : Rel T}
 
-lemma star.singleton {x y} : e x y -> star e x y := by
+theorem star.singleton {x y} : e x y -> star e x y := by
   intro h
   apply star.SE
   apply star.R
   assumption
 
-lemma star.trans {y x z} : star e x y -> star e y z -> star e x z := by
+theorem star.trans {y x z} : star e x y -> star e y z -> star e x z := by
   intros h1 h2
   induction h2 with
   | R => exact h1
   | SE _ rel ih => apply star.SE ih rel
 
-lemma star.ES {x y z} : e x y -> star e y z -> star e x z := by
+theorem star.ES {x y z} : e x y -> star e y z -> star e x z := by
   intro h
   apply star.trans
   apply star.singleton
   assumption
 
-lemma star.conv {x y} : star e x y -> conv e x y := by
+theorem star.conv {x y} : star e x y -> conv e x y := by
   intro h
   induction h with
   | R => constructor
   | SE _ rel ih => apply conv.SE ih rel
 
-lemma star.img {T1 T2} {f : T1 -> T2} {e1 e2} :
+theorem star.img {T1 T2} {f : T1 -> T2} {e1 e2} :
   (∀ {x y}, e1 x y -> star e2 (f x) (f y)) ->
   (∀ {x y}, star e1 x y -> star e2 (f x) (f y)) := by
   intros h1 x y h2
   induction h2 with
-  | R => aesop
+  | R => constructor
   | @SE y z _ rel ih => apply star.trans ih (h1 rel)
 
-lemma star.hom {T1 T2} (f : T1 -> T2) {e1 e2} :
+theorem star.hom {T1 T2} (f : T1 -> T2) {e1 e2} :
   (∀ {x y}, e1 x y -> e2 (f x) (f y)) ->
   (∀ {x y}, star e1 x y -> star e2 (f x) (f y)) := by
   intro h; apply star.img
   intros x y h0
-  apply h at h0
-  apply star.singleton h0
+  specialize h h0
+  apply star.singleton h
 
-lemma star.closure {T} {e1 e2 : Rel T} : e1 <=2 star e2 -> star e1 <=2 star e2 := by
+theorem star.closure {T} {e1 e2 : Rel T} : e1 <=2 star e2 -> star e1 <=2 star e2 := by
   apply star.img
 
-lemma star.monotone {T} {e1 e2 : Rel T} : e1 <=2 e2 -> star e1 <=2 star e2 := by
+theorem star.monotone {T} {e1 e2 : Rel T} : e1 <=2 e2 -> star e1 <=2 star e2 := by
   intro h1; apply star.closure
   intros x y h2
-  apply h1 at h2
-  apply star.singleton h2
+  specialize h1 h2
+  apply star.singleton h1
 
-lemma conv.singleton {x y} : e x y -> conv e x y := by
+theorem conv.singleton {x y} : e x y -> conv e x y := by
   intro h; apply conv.SE conv.R h
 
-lemma conv.singletoni {x y} : e y x -> conv e x y := by
+theorem conv.singletoni {x y} : e y x -> conv e x y := by
   intro h; apply conv.SEi conv.R h
 
-lemma conv.trans {y x z} : conv e x y -> conv e y z -> conv e x z := by
+theorem conv.trans {y x z} : conv e x y -> conv e y z -> conv e x z := by
   intros h1 h2
   induction h2 with
   | R => exact h1
   | SE _ rel ih => apply conv.SE ih rel
   | SEi _ rel ih => apply conv.SEi ih rel
 
-lemma conv.ES {x y z} : e x y -> conv e y z -> conv e x z := by
+theorem conv.ES {x y z} : e x y -> conv e y z -> conv e x z := by
   intro h
   apply conv.trans
   apply conv.singleton
   assumption
 
-lemma conv.ESi {x y z} : e y x -> conv e y z -> conv e x z := by
+theorem conv.ESi {x y z} : e y x -> conv e y z -> conv e x z := by
   intro h
   apply conv.trans
   apply conv.singletoni
   assumption
 
-lemma conv.sym {x y} : conv e x y -> conv e y x := by
+theorem conv.sym {x y} : conv e x y -> conv e y x := by
   intro h
   induction h with
   | R => constructor
   | SE _ rel ih => apply conv.ESi rel ih
   | SEi _ rel ih => apply conv.ES rel ih
 
-lemma conv.join {x y z} : star e x y -> star e z y -> conv e x z := by
+theorem conv.join {x y z} : star e x y -> star e z y -> conv e x z := by
   intro h1 h2
   apply conv.trans
   apply star.conv h1
   apply conv.sym
   apply star.conv h2
 
-lemma conv.img {T1 T2} {f : T1 -> T2} {e1 e2} :
+theorem conv.img {T1 T2} {f : T1 -> T2} {e1 e2} :
   (∀ {x y}, e1 x y -> conv e2 (f x) (f y)) ->
   (∀ {x y}, conv e1 x y -> conv e2 (f x) (f y)) := by
   intros h1 x y h2
   induction h2 with
-  | R => aesop
+  | R => constructor
   | SE _ rel ih =>
     apply conv.trans ih (h1 rel)
   | SEi _ rel ih =>
@@ -134,19 +130,21 @@ lemma conv.img {T1 T2} {f : T1 -> T2} {e1 e2} :
     apply conv.sym
     apply h1 rel
 
-lemma conv.hom {T1 T2} (f : T1 -> T2) {e1 e2} :
+theorem conv.hom {T1 T2} (f : T1 -> T2) {e1 e2} :
   (∀ {x y}, e1 x y -> e2 (f x) (f y)) ->
   (∀ {x y}, conv e1 x y -> conv e2 (f x) (f y)) := by
   intro h; apply conv.img
   intros x y h0
-  apply h at h0
-  apply conv.singleton h0
+  specialize h h0
+  apply conv.singleton h
 
-lemma confluent_cr : confluent e <-> CR e := by
+theorem confluent_cr : confluent e <-> CR e := by
   constructor
   . intro h1 x y h2
     induction h2 with
-    | R => exists x; constructor <;> aesop
+    | R =>
+      exists x
+      constructor <;> constructor
     | @SE y z _ rel ih =>
       rcases ih with ⟨u, ⟨h2, h3⟩⟩
       rcases h1 h3 (star.singleton rel) with ⟨v, ⟨h4, h5⟩⟩
@@ -159,15 +157,20 @@ lemma confluent_cr : confluent e <-> CR e := by
       . apply h2
       . apply star.ES rel h3
   . intro h x y z  h1 h2
-    apply star.conv at h1
-    apply star.conv at h2
+    have h1 := star.conv h1
+    have h2 := star.conv h2
     apply h
     apply conv.trans (conv.sym h1) h2
 
-lemma com.strip {e1 e2 : Rel T} : com e1 e2 -> com (star e2) e1 := by
+theorem com.strip {e1 e2 : Rel T} : com e1 e2 -> com (star e2) e1 := by
   intros h1 x y z h2
   induction h2 with
-  | R => intro h2; exists z; aesop
+  | R =>
+    intro h2
+    exists z
+    constructor
+    . assumption
+    . constructor
   | SE _ rel2 ih =>
     intro h2
     rcases ih h2 with ⟨u, ⟨rel1, h3⟩⟩
@@ -176,12 +179,12 @@ lemma com.strip {e1 e2 : Rel T} : com e1 e2 -> com (star e2) e1 := by
     . assumption
     . apply star.SE h3 rel2
 
-lemma com.lift {e1 e2 : Rel T} : com e1 e2 -> com (star e1) (star e2) := by
+theorem com.lift {e1 e2 : Rel T} : com e1 e2 -> com (star e1) (star e2) := by
   intro h
-  apply com.strip at h
-  apply com.strip at h
+  have h := @com.strip _ e1 e2 h
+  have h := @com.strip _ (star e2) e1 h
   assumption
 
-lemma diamond_confluent : diamond e -> confluent e := by
+theorem diamond_confluent : diamond e -> confluent e := by
   apply com.lift
 end ars_lemmas
