Lamcalc/Syntax.lean
@@ -13,8 +13,7 @@ inductive tm where
 instance : Ids tm where
   ids := tm.var
 
-@[simp]
-lemma ids_var x : tm.var x = ids x := rfl
+@[simp] theorem ids_var x : tm.var x = ids x := rfl
 
 def tm.rename (ξ : Nat -> Nat) (m : tm) : tm :=
   match m with
@@ -26,11 +25,10 @@ def tm.rename (ξ : Nat -> Nat) (m : tm) : tm :=
 instance : Rename tm where
   rename := tm.rename
 
-lemma rename_ids ξ x : rename ξ (ids x) = @ids tm _ (ξ x) := rfl
-lemma rename_lam ξ a m : rename ξ (tm.lam a m) = tm.lam a (rename (upren ξ) m) := rfl
-lemma rename_app ξ m n : rename ξ (tm.app m n) = tm.app (rename ξ m) (rename ξ n) := rfl
-lemma rename_unit ξ : rename ξ (tm.unit) = tm.unit := rfl
-attribute [simp] rename_ids rename_lam rename_app rename_unit
+@[simp] theorem rename_ids ξ x : rename ξ (ids x) = @ids tm _ (ξ x) := rfl
+@[simp] theorem rename_lam ξ a m : rename ξ (tm.lam a m) = tm.lam a (rename (upren ξ) m) := rfl
+@[simp] theorem rename_app ξ m n : rename ξ (tm.app m n) = tm.app (rename ξ m) (rename ξ n) := rfl
+@[simp] theorem rename_unit ξ : rename ξ (tm.unit) = tm.unit := rfl
 
 def tm.subst (σ : Nat -> tm) (m : tm) : tm :=
   match m with
@@ -42,33 +40,33 @@ def tm.subst (σ : Nat -> tm) (m : tm) : tm :=
 instance : Subst tm where
   subst := tm.subst
 
-lemma subst_ids (σ : Nat -> tm) x : subst σ (ids x) = σ x := rfl
-lemma subst_lam σ a m : subst σ (tm.lam a m) = tm.lam a (subst (up σ) m) := rfl
-lemma subst_app σ m n : subst σ (tm.app m n) = tm.app (subst σ m) (subst σ n) := rfl
-lemma subst_unit σ : subst σ tm.unit = tm.unit := rfl
-attribute [simp] subst_ids subst_lam subst_app subst_unit
+@[simp] theorem subst_ids (σ : Nat -> tm) x : subst σ (ids x) = σ x := by rfl
+@[simp] theorem subst_lam σ a m : subst σ (tm.lam a m) = tm.lam a (subst (up σ) m) := by rfl
+@[simp] theorem subst_app σ m n : subst σ (tm.app m n) = tm.app (subst σ m) (subst σ n) := by rfl
+@[simp] theorem subst_unit σ : subst σ tm.unit = tm.unit := rfl
 
-@[simp]
-lemma up_upren (ξ : Nat -> Nat) :
+theorem up_upren (ξ : Nat -> Nat) :
   @up tm _ _ (ren ξ) = ren (upren ξ) := by
   apply funext
   intro x
   cases x with
   | zero => simp [upren, up, ren, scons, funcomp]
-  | succ n => simp [upren, up, ren, scons, funcomp]
+  | succ => simp [upren, up, ren, scons, funcomp]
 
-@[simp]
-lemma up_upren_n (ξ : Nat -> Nat) (n : Nat) :
-  @upn tm _ _ n (ren ξ ) = ren (upren^[n] ξ) := by
+theorem up_upren_n (ξ : Nat -> Nat) (n : Nat) :
+  @upn tm _ _ n (ren ξ ) = ren (n.repeat upren ξ) := by
   induction n generalizing ξ with
-  | zero => simp [upn]
-  | succ n ih => simp; rw [ih]
+  | zero => simp [upn, Nat.repeat]
+  | succ n ih =>
+    simp[upn, Nat.repeat];
+    rw [<-up_upren]
+    rw [<-ih, <-upn]
 
-@[simp]
-lemma rename_subst ξ (m : tm) : rename ξ m = m.[ren ξ] := by
+@[simp] theorem rename_subst ξ (m : tm) : rename ξ m = m.[ren ξ] := by
   induction m generalizing ξ with
   | var x => simp [ren, funcomp]
-  | lam a m ih => simp; rw[ih]
+  | lam a m ih =>
+    simp[up_upren]; rw[ih]
   | app m n ihm ihn =>
     simp
     constructor
@@ -76,32 +74,76 @@ lemma rename_subst ξ (m : tm) : rename ξ m = m.[ren ξ] := by
     . apply ihn
   | _ => simp
 
-@[simp]
-lemma up_id : @up tm _ _ ids = ids := by
+@[simp] theorem up_shift (σ : Nat -> tm) :
+  up σ = ids 0 .: (σ @@ shift) := by
+  simp [up, scomp]
   apply funext
   intro x
   cases x with
-  | zero => simp [up, scons]
-  | succ n => simp [up, scons, ren, funcomp]
+  | zero => simp[scons]
+  | succ x =>
+    simp [scons, funcomp]
+    simp [rename_subst, shift]
 
-@[simp]
-lemma up_id_n n : @upn tm _ _ n ids = ids := by
-  induction n with
+open Lean Elab Macro
+syntax "asimp" : tactic
+syntax "asimp" "at" ident : tactic
+macro_rules
+| `(tactic| asimp) =>
+  `(tactic| simp; repeat rw [<-up_shift])
+| `(tactic| asimp at $x:ident) =>
+  `(tactic| simp at $x:ident; repeat rw [<-up_shift] at $x:ident)
+
+@[simp] theorem ids_comp (σ : Nat -> tm) : ids @@ σ = σ := by rfl
+@[simp] theorem ids_shift : (@ids tm _ 0) .: shift = ids := by
+  apply funext
+  intro x
+  cases x with
+  | zero => simp[scons]
+  | succ x => simp[scons, shift, ren, funcomp]
+
+@[simp] theorem shift_scomp (m : tm) (σ : Nat -> tm) :
+  shift @@ (m .: σ) = σ := by
+  apply funext
+  intro x
+  simp[shift, ren]
+  simp[funcomp, scomp, scons]
+
+@[simp] theorem ids0_scons (σ : Nat -> tm) :
+  (ids 0).[σ] .: (shift @@ σ) = σ := by
+  apply funext
+  intro x
+  simp[scons]
+  cases x with
   | zero => simp
-  | succ n ihn => simp; exact ihn
+  | succ => simp[scomp, funcomp, shift, ren]
 
-@[simp]
-lemma subst_id (m : tm) : m.[ids] = m := by
-  induction m <;> simp
-  case lam a m ih => exact ih
-  case app m n ihm ihn =>
-    constructor <;> aesop
+@[simp] theorem subst_id (m : tm) :
+  m.[ids] = m := by
+  induction m with
+  | var x => simp
+  | lam a m ih =>
+    simp
+    assumption
+  | app m n ih1 ih2 =>
+    simp
+    constructor <;> assumption
+  | unit => simp
 
-@[simp]
-lemma id_subst (σ : Nat -> tm) x : (ids x).[σ] = σ x := rfl
+@[simp] theorem comp_ids (σ : Nat -> tm) : σ @@ ids = σ := by
+  apply funext
+  intro x
+  simp[scomp, funcomp]
 
-@[simp]
-lemma up_comp_ren_subst {T} [Ids T] [Rename T] (ξ : Nat -> Nat) (σ : Nat -> T) :
+@[simp] theorem scons_scomp m (σ τ : Nat -> tm) :
+  (m .: σ) @@ τ = m.[τ] .: σ @@ τ := by
+  apply funext
+  intro x
+  cases x with
+  | zero => simp[scomp, funcomp, scons]
+  | succ => simp[scomp, funcomp, scons]
+
+theorem up_comp_ren_subst {T} [Ids T] [Rename T] (ξ : Nat -> Nat) (σ : Nat -> T) :
   up (ξ @@@ σ) = upren ξ @@@ up σ := by
   apply funext
   intro x
@@ -109,19 +151,20 @@ lemma up_comp_ren_subst {T} [Ids T] [Rename T] (ξ : Nat -> Nat) (σ : Nat -> T)
   | zero => rfl
   | succ n => simp [up, scons, upren, funcomp]
 
-@[simp]
-lemma ren_subst_comp ξ σ (m : tm) : (rename ξ m).[σ] = m.[ξ @@@ σ] := by
+theorem ren_subst_comp ξ σ (m : tm) : m.[ren ξ].[σ] = m.[ξ @@@ σ] := by
   induction m generalizing ξ σ with
   | var x => rfl
-  | lam a m ih => simp; rw [<- ih]; simp
+  | lam a m ih =>
+    simp [up_comp_ren_subst]
+    rw [<- ih]
+    simp [<- up_upren]
   | app m n ihm ihn =>
     simp; constructor
-    . rw [<- ihm]; simp
-    . rw [<- ihn]; simp
+    . rw [<- ihm]
+    . rw [<- ihn]
   | unit => simp
 
-@[simp]
-lemma up_comp_subst_ren (σ : Nat -> tm) (ξ : Nat -> Nat) :
+theorem up_comp_subst_ren (σ : Nat -> tm) (ξ : Nat -> Nat) :
   up (σ @@@ rename ξ) = up σ @@@ rename (upren ξ) := by
   apply funext
   intro x
@@ -133,48 +176,49 @@ lemma up_comp_subst_ren (σ : Nat -> tm) (ξ : Nat -> Nat) :
     have h2 := ren_subst_comp ξ (ren Nat.succ) (σ n); simp at h2
     rw [h1, h2]; rfl
 
-@[simp]
-lemma subst_ren_comp σ ξ (m : tm) : rename ξ m.[σ] = m.[σ @@@ rename ξ] := by
+theorem subst_ren_comp σ ξ (m : tm) : m.[σ].[ren ξ] = m.[σ @@@ rename ξ] := by
   induction m generalizing σ ξ with
-  | var x => rfl
-  | lam a m ih => simp; rw [<- ih]; simp
+  | var x => simp
+  | lam a m ih =>
+    asimp;
+    rw [up_upren]
+    rw [ih]
+    rw [<- up_comp_subst_ren]
   | app m n ihm ihn =>
     simp; constructor
-    . rw [<- ihm]; simp
-    . rw [<- ihn]; simp
+    . rw [<- ihm]
+    . rw [<- ihn]
   | unit => rfl
 
-@[simp]
-lemma up_comp (σ τ : Nat -> tm) : up (σ @@ τ) = up σ @@ up τ := by
+theorem up_comp (σ τ : Nat -> tm) : up (σ @@ τ) = up σ @@ up τ := by
   apply funext
   intro x
   cases x with
-  | zero => simp [scomp, funcomp]
+  | zero =>
+    simp [up, scons, scomp, funcomp]
   | succ n =>
     simp [up, scons, scomp, funcomp]
-    rw [<- up]
-    have h1 := subst_ren_comp τ Nat.succ (σ n); simp at h1
-    have h2 := ren_subst_comp Nat.succ (up τ) (σ n); simp at h2
-    rw [h1, h2]; rfl
+    rw[<-up]
+    have h1 := subst_ren_comp τ Nat.succ (σ n)
+    have h2 := ren_subst_comp Nat.succ (up τ) (σ n)
+    rw [h1, h2]
+    rfl
 
-@[simp]
-lemma subst_comp (σ τ : Nat -> tm) m : m.[σ].[τ] = m.[σ @@ τ] := by
+@[simp] theorem subst_comp (σ τ : Nat -> tm) m : m.[σ].[τ] = m.[σ @@ τ] := by
   induction m generalizing σ τ with
   | var x => simp [scomp, funcomp]
-  | lam a m ih => simp; rw [ih]
+  | lam a m ih =>
+    asimp
+    rw [ih]
+    rw [up_comp]
   | app m n ihm ihn =>
     simp; constructor
     . apply ihm
     . apply ihn
   | unit => rfl
 
-@[simp]
-lemma up_comp_subst (m : tm) (σ : Nat -> tm) :
-  up σ @@ (m.[σ] .: ids) = (m .: ids) @@ σ := by
-  apply funext; intro x
-  cases x with
-  | zero => simp [scomp, funcomp, scons]
-  | succ n =>
-    simp [scomp, funcomp, scons, up]
-    have h : ren Nat.succ @@@ subst (m.[σ] .: ids) = ids := rfl
-    rw [h]; simp
+@[simp] theorem scomp_assoc (σ τ θ : Nat -> tm) :
+  (σ @@ τ) @@ θ = σ @@ (τ @@ θ) := by
+  apply funext
+  intro x
+  simp[scomp, funcomp]
